ExistentialRules/Terms/Cyclic.lean
@@ -1,4 +1,7 @@
-import ExistentialRules.Terms.Basic
+module
+
+import BasicLeanDatastructures.List.Basic
+public import ExistentialRules.Terms.Basic
 
 /-!
 # Cyclic Terms
@@ -29,63 +32,24 @@ def contains_func (func : SkolemFS sig) : FiniteTree (SkolemFS sig) sig.C -> Boo
 | .inner func' ts => func == func' || ts.attach.any (fun ⟨t, _⟩ => contains_func func t)
 
 /-- A `PreGroundTerm` is `cyclic` if one of its children `contains_func` the function symbol of the term or if one of its children is already `cyclic`. Constants are never cyclic. -/
-def cyclic : FiniteTree (SkolemFS sig) sig.C -> Bool
+public def cyclic : FiniteTree (SkolemFS sig) sig.C -> Bool
 | .leaf _ => false
 | .inner func ts => ts.any (contains_func func) || ts.attach.any (fun ⟨t, _⟩ => PreGroundTerm.cyclic t)
 
 /-- All elements of the `function_paths` paths are inner labels of the finite tree. -/
-theorem function_path_elements_are_inner_labels (t : FiniteTree (SkolemFS sig) sig.C) : ∀ (path : List (SkolemFS sig)), path ∈ PreGroundTerm.function_paths t -> ∀f, f ∈ path -> f ∈ t.innerLabels := by
+theorem function_path_elements_are_inner_labels (t : FiniteTree (SkolemFS sig) sig.C) :
+    ∀ (path : List (SkolemFS sig)), path ∈ function_paths t -> ∀f, f ∈ path -> f ∈ t.innerLabels := by
   intro path path_mem f f_mem
-  induction t generalizing path with
-  | leaf c =>
-    simp only [function_paths, List.mem_singleton] at path_mem
-    rw [path_mem] at f_mem
-    simp at f_mem
-  | inner func ts ih =>
-    unfold function_paths at path_mem
-    cases ts with
-    | nil =>
-      simp only [↓reduceIte] at path_mem
-      rw [List.mem_singleton] at path_mem
-      rw [path_mem] at f_mem
-      rw [List.mem_singleton] at f_mem
-      unfold FiniteTree.innerLabels
-      rw [List.mem_cons]
-      apply Or.inl
-      exact f_mem
-    | cons hd tl =>
-      simp only [List.cons_ne_nil, ↓reduceIte] at path_mem
-      rw [List.map_flatMap, List.mem_flatMap] at path_mem
-      rcases path_mem with ⟨t, t_mem, path_mem⟩
-      rw [List.mem_map] at path_mem
-      rcases path_mem with ⟨path', mem, eq⟩
-      rw [← eq] at f_mem
-      rw [List.mem_cons] at f_mem
-      unfold FiniteTree.innerLabels
-      rw [List.mem_cons]
-      cases f_mem with
-      | inl f_mem => apply Or.inl; exact f_mem
-      | inr f_mem =>
-        apply Or.inr
-        rw [List.mem_flatMap]
-        exists t
-        constructor
-        . exact t_mem
-        . exact ih t t_mem path' mem f_mem
+  fun_induction function_paths generalizing path <;> (unfold FiniteTree.innerLabels; grind)
 
 /-- There is a path in `function_paths` that matches the depth of the term (-1). That means that this path is one of maximal possible length. -/
-theorem function_path_of_depth_exists (t : FiniteTree (SkolemFS sig) sig.C) : ∃ (path : List (SkolemFS sig)), path ∈ PreGroundTerm.function_paths t ∧ path.length = t.depth - 1 := by
+theorem function_path_of_depth_exists (t : FiniteTree (SkolemFS sig) sig.C) :
+    ∃ (path : List (SkolemFS sig)), path ∈ function_paths t ∧ path.length = t.depth - 1 := by
   induction t with
   | leaf c => exists []; simp [FiniteTree.depth, function_paths]
   | inner f ts ih =>
     cases ts with
-    | nil =>
-      exists [f]
-      constructor
-      . unfold function_paths
-        simp
-      . unfold FiniteTree.depth
-        simp
+    | nil => exists [f]; simp [FiniteTree.depth, function_paths]
     | cons hd tl =>
       have : ∃ t, t ∈ (hd::tl) ∧ t.depth = (FiniteTree.inner f (hd :: tl)).depth - 1 := by
         simp only [FiniteTree.depth]
@@ -97,84 +61,39 @@ theorem function_path_of_depth_exists (t : FiniteTree (SkolemFS sig) sig.C) : �
       rcases ih t t_mem with ⟨path, mem, len⟩
       exists (f :: path)
       constructor
-      . unfold function_paths
-        simp only [List.cons_ne_nil, ↓reduceIte]
-        rw [List.mem_map]
-        exists path
-        constructor
-        . rw [List.mem_flatMap]
-          exists t
-        . rfl
+      . unfold function_paths; grind
       . rw [← t_depth, List.length_cons]
         rw [len]
         rw [Nat.sub_one_add_one]
         intro contra
-        cases t with
-        | leaf _ => simp [FiniteTree.depth] at contra
-        | inner _ _ => simp [FiniteTree.depth] at contra
+        cases t <;> simp [FiniteTree.depth] at contra
 
 /-- For each element in a path from `function_paths`, `contains_func` is true. -/
-theorem function_path_elements_are_in_contains_func (t : FiniteTree (SkolemFS sig) sig.C) : ∀ (path : List (SkolemFS sig)), path ∈ PreGroundTerm.function_paths t -> ∀ f, f ∈ path -> PreGroundTerm.contains_func f t := by
+theorem function_path_elements_are_in_contains_func (t : FiniteTree (SkolemFS sig) sig.C) :
+    ∀ (path : List (SkolemFS sig)), path ∈ function_paths t -> ∀ f, f ∈ path -> contains_func f t := by
   intro path path_mem f f_mem
-  induction t generalizing path with
-  | leaf c =>
-    simp only [function_paths, List.mem_singleton] at path_mem
-    rw [path_mem] at f_mem
-    simp at f_mem
-  | inner func ts ih =>
-    unfold contains_func
-    rw [Bool.or_eq_true]
-    unfold function_paths at path_mem
-    cases ts with
-    | nil =>
-      simp only [↓reduceIte] at path_mem
-      rw [List.mem_singleton] at path_mem
-      rw [path_mem] at f_mem
-      rw [List.mem_singleton] at f_mem
-      apply Or.inl
-      rw [f_mem]
-      simp
-    | cons hd tl =>
-      simp only [List.cons_ne_nil, ↓reduceIte] at path_mem
-      rw [List.map_flatMap, List.mem_flatMap] at path_mem
-      rcases path_mem with ⟨t, t_mem, path_mem⟩
-      rw [List.mem_map] at path_mem
-      rcases path_mem with ⟨path', mem, eq⟩
-      rw [← eq] at f_mem
-      rw [List.mem_cons] at f_mem
-      cases f_mem with
-      | inl f_mem => apply Or.inl; rw [f_mem]; simp
-      | inr f_mem =>
-        apply Or.inr
-        rw [List.any_eq_true]
-        exists ⟨t, t_mem⟩
-        constructor
-        . apply List.mem_attach
-        . exact ih t t_mem path' mem f_mem
+  fun_induction function_paths generalizing path
+  . grind
+  . unfold contains_func; grind
+  . unfold contains_func; simp; grind
 
 /-- A term is `cyclic` if a path in `function_paths` has a duplicate. -/
-theorem cyclic_of_path_with_dup (t : FiniteTree (SkolemFS sig) sig.C) (path : List (SkolemFS sig)) (path_mem : path ∈ PreGroundTerm.function_paths t) (dup : ¬ path.Nodup) : PreGroundTerm.cyclic t := by
+theorem cyclic_of_path_with_dup
+    (t : FiniteTree (SkolemFS sig) sig.C)
+    (path : List (SkolemFS sig)) (path_mem : path ∈ function_paths t) (dup : ¬ path.Nodup) : cyclic t := by
   induction t generalizing path with
-  | leaf c =>
-    unfold PreGroundTerm.function_paths at path_mem
-    rw [List.mem_singleton] at path_mem
-    rw [path_mem] at dup
-    simp at dup
+  | leaf _ => unfold function_paths at path_mem; grind
   | inner f ts ih =>
-    unfold PreGroundTerm.function_paths at path_mem
+    unfold function_paths at path_mem
     cases ts with
-    | nil =>
-      simp only [↓reduceIte] at path_mem
-      rw [List.mem_singleton] at path_mem
-      rw [path_mem] at dup
-      simp at dup
+    | nil => grind
     | cons hd tl =>
       simp only [List.cons_ne_nil, ↓reduceIte] at path_mem
       rw [List.map_flatMap, List.mem_flatMap] at path_mem
       rcases path_mem with ⟨t, t_mem, path_mem⟩
       rw [List.mem_map] at path_mem
       rcases path_mem with ⟨path', mem, eq⟩
-      unfold PreGroundTerm.cyclic
+      unfold cyclic
       rw [Bool.or_eq_true]
       cases Decidable.em (f ∈ path') with
       | inl f_mem =>
@@ -199,29 +118,21 @@ theorem cyclic_of_path_with_dup (t : FiniteTree (SkolemFS sig) sig.C) (path : Li
 variable [DecidableEq sig.C]
 
 /-- Consider a (deduplicated) list of possible function symbols and a term. If the depth of the term is at least the number of function symbols + 2, then the term must be cyclic.  -/
-theorem cyclic_of_depth_too_big (t : PreGroundTerm sig) (funcs : List (SkolemFS sig)) (nodup : funcs.Nodup) (funcs_in_t_from_funcs : ∀ func, func ∈ t.innerLabels -> func ∈ funcs) : funcs.length + 2 ≤ t.depth -> PreGroundTerm.cyclic t := by
+public theorem cyclic_of_depth_too_big (t : PreGroundTerm sig)
+    (funcs : List (SkolemFS sig)) (nodup : funcs.Nodup) (funcs_in_t_from_funcs : ∀ func, func ∈ t.innerLabels -> func ∈ funcs) :
+    funcs.length + 2 ≤ t.depth -> cyclic t := by
   intro le_depth
-  have := PreGroundTerm.function_path_of_depth_exists t
-  rcases this with ⟨path, path_mem, path_len⟩
+  rcases function_path_of_depth_exists t with ⟨path, path_mem, path_len⟩
 
-  have path_length_gt : funcs.length < path.length := by
-    rw [path_len]
-    apply Nat.lt_of_succ_le
-    apply Nat.le_of_succ_le_succ
-    rw [Nat.succ_eq_add_one]
-    rw [Nat.succ_eq_add_one]
-    rw [Nat.sub_one_add_one]
-    . exact le_depth
-    . unfold FiniteTree.depth
-      cases t <;> simp
+  have path_length_gt : funcs.length < path.length := by grind
 
   have dup_in_path : ¬ path.Nodup := by
     apply List.contains_dup_of_exceeding_nodup_list_with_same_elements funcs path nodup path_length_gt
     intro f f_mem
     apply funcs_in_t_from_funcs
-    exact PreGroundTerm.function_path_elements_are_inner_labels t path path_mem f f_mem
+    exact function_path_elements_are_inner_labels t path path_mem f f_mem
 
-  exact PreGroundTerm.cyclic_of_path_with_dup t path path_mem dup_in_path
+  exact cyclic_of_path_with_dup t path path_mem dup_in_path
 
 end PreGroundTerm
 
