ExistentialRules/Terms/ListsOfTerms.lean
@@ -1,5 +1,7 @@
-import BasicLeanDatastructures.List.AllListsOfLength
-import ExistentialRules.Terms.Basic
+module
+
+public import BasicLeanDatastructures.List.AllListsOfLength
+public import ExistentialRules.Terms.Basic
 
 /-!
 # Computing all GroundTerms of a given depth
@@ -13,7 +15,7 @@ This is required for MFA later since we want to argue that when a rule set is MF
 variable {sig : Signature} [DecidableEq sig.C] [DecidableEq sig.V]
 
 /-- We recursively construct all `GroundTerm`s that have at most a given depth. For example, the terms with at most depth 1 are exactly the constants. The recursion step uses all terms that have at most the previous depth and then combines them in all possible ways using each of the available function symbols as the new root. -/
-def all_terms_limited_by_depth (constants : List sig.C) (funcs : List (SkolemFS sig)) : Nat -> List (GroundTerm sig)
+public def all_terms_limited_by_depth (constants : List sig.C) (funcs : List (SkolemFS sig)) : Nat -> List (GroundTerm sig)
 | 0 => []
 | 1 => constants.map GroundTerm.const
 | .succ (.succ depth) =>
@@ -28,43 +30,24 @@ def all_terms_limited_by_depth (constants : List sig.C) (funcs : List (SkolemFS 
   ) ++ prev
 
 /-- This theorem expresses the desired property of the definition above. The constructed list of `GroundTerm`s contains exactly the terms that have at most the desired depth and feature only constants and function symbols from the allowed lists. This theorem is at the same time a sanity check that our definition above is behaving as expected. -/
-theorem mem_all_terms_limited_by_depth (constants : List sig.C) (funcs : List (SkolemFS sig)) (depth : Nat) :
-    ∀ t, t ∈ (all_terms_limited_by_depth constants funcs depth) ↔ (t.depth ≤ depth ∧ (∀ c, c ∈ t.constants -> c ∈ constants) ∧ (∀ func, func ∈ t.functions -> func ∈ funcs)) := by
-  induction depth with
-  | zero =>
-    simp [all_terms_limited_by_depth]
-    intro t _ t_depth
-    cases t <;> simp [GroundTerm.depth, FiniteTree.depth] at t_depth
-  | succ depth ih =>
-    intro t
-    unfold all_terms_limited_by_depth
-
-    cases depth with
-    | zero =>
-      simp only [Nat.zero_add]
-      constructor
-      . intro h
-        rw [List.mem_map] at h
-        rcases h with ⟨c, c_mem, h⟩
-        rw [← h]
-        rw [GroundTerm.depth_const]
-        rw [GroundTerm.constants_const]
-        rw [GroundTerm.functions_const]
-        simp [c_mem]
-      . intro h
-        cases eq : t with
-        | const c =>
-          rw [List.mem_map]
-          exists c
-          constructor
-          . apply h.right.left
-            simp [eq, GroundTerm.constants_const]
-          . rfl
-        | func _ ts _ =>
-          have contra := h.left
-          rw [eq, GroundTerm.depth_func] at contra
+public theorem mem_all_terms_limited_by_depth (constants : List sig.C) (funcs : List (SkolemFS sig)) (depth : Nat) :
+    ∀ t, t ∈ (all_terms_limited_by_depth constants funcs depth) ↔
+      (t.depth ≤ depth ∧ (∀ c, c ∈ t.constants -> c ∈ constants) ∧ (∀ func, func ∈ t.functions -> func ∈ funcs)) := by
+  fun_induction all_terms_limited_by_depth
+  . intro t
+    have : t.depth ≠ 0 := by apply Nat.ne_zero_of_lt; exact GroundTerm.depth_gt_zero
+    simp [this]
+  . intro t
+    constructor
+    . grind
+    . intro h
+      cases eq : t with
+      | const _ => grind
+      | func _ ts _ =>
+        have : t.depth > 1 := by
+          rw [eq, GroundTerm.depth_func]
           cases eq : (ts.map GroundTerm.depth).max? with
-          | none => simp [eq] at contra
+          | none => simp
           | some m =>
             cases m with
             | zero =>
@@ -72,188 +55,91 @@ theorem mem_all_terms_limited_by_depth (constants : List sig.C) (funcs : List (S
               have contra := eq.left
               rw [List.mem_map] at contra
               rcases contra with ⟨t, t_mem, contra⟩
-              cases t <;> simp [GroundTerm.depth_const, GroundTerm.depth_func] at contra
-            | succ m =>
-              rw [eq, Nat.add_comm] at contra
-              simp at contra
+              have : t.depth ≠ 0 := by apply Nat.ne_zero_of_lt; exact GroundTerm.depth_gt_zero
+              apply False.elim; apply this; exact contra
+            | succ m => simp
+        grind
+  case case3 depth prev ih =>
+    intro t
+    have aux : ∀ (ts : List (GroundTerm sig)),
+      ((∀ (t : GroundTerm sig), t ∈ ts -> t ∈ (all_terms_limited_by_depth constants funcs depth.succ)) ↔
+      ((ts.all (fun t => t.depth ≤ depth.succ)) ∧ (∀ c, c ∈ (ts.flatMap GroundTerm.constants) -> c ∈ constants) ∧
+      (∀ func, func ∈ (ts.flatMap GroundTerm.functions) -> func ∈ funcs))) := by grind
+    constructor
+    . intro h
+      rw [List.mem_append] at h
+      cases h with
+      | inr h => grind
+      | inl h =>
+        simp only [List.mem_flatMap, List.mem_map] at h
+        rcases h with ⟨func, func_mem, ts, ts_mem, t_eq⟩
+        rw [← t_eq]
+        unfold List.attach at ts_mem
+        unfold List.attachWith at ts_mem
+        rw [List.mem_pmap] at ts_mem
+        rcases ts_mem with ⟨ts_val, ts_mem, ts_eq⟩
+        rw [mem_all_lists_of_length] at ts_mem
 
-    | succ depth =>
-      have aux : ∀ (ts : List (GroundTerm sig)),
-          ((∀ (t : GroundTerm sig), t ∈ ts -> t ∈ (all_terms_limited_by_depth constants funcs depth.succ)) ↔
-          ((ts.all (fun t => t.depth ≤ depth.succ)) ∧ (∀ c, c ∈ (ts.flatMap GroundTerm.constants) -> c ∈ constants) ∧ (∀ func, func ∈ (ts.flatMap GroundTerm.functions) -> func ∈ funcs))) := by
-        intro ts
-        induction ts with
-        | nil => simp
-        | cons hd tl ih_inner =>
-          simp only [List.mem_cons, List.all_cons, Bool.and_eq_true, decide_eq_true_eq, List.flatMap_cons, List.mem_append]
-          constructor
-          . intro h
-            have ih := (ih hd).mp (by apply h; simp)
-            have ih_inner := ih_inner.mp (by intro _ t_mem; apply h; apply Or.inr; exact t_mem)
+        rw [GroundTerm.depth_func]
+        rw [GroundTerm.constants_func]
+        rw [GroundTerm.functions_func]
+
+        have aux := (aux ts_val).mp (by
+          intro t t_mem
+          apply ts_mem.right
+          exact t_mem
+        )
+
+        rw [← ts_eq]
+        constructor
+        . rw [Nat.add_comm]
+          apply Nat.succ_le_succ
+          cases eq : (ts_val.map GroundTerm.depth).max? with
+          | none => simp
+          | some m =>
+            rw [Option.getD_some, (ts_val.map GroundTerm.depth).max?_le_iff]
+            . grind
+            . grind
+        . grind
+
+    . intro h
+      rw [List.mem_append]
+      simp only [List.mem_flatMap, List.mem_map]
+      rcases h with ⟨depth_le, consts_mem, funcs_mem⟩
+      rw [Nat.le_iff_lt_or_eq] at depth_le
+      cases depth_le with
+      | inl depth_le => grind
+      | inr depth_le =>
+        cases eq : t with
+        | const _ => grind
+        | func t_func ts =>
+          rw [eq, GroundTerm.depth_func] at depth_le
+          rw [eq, GroundTerm.constants_func] at consts_mem
+          rw [eq, GroundTerm.functions_func] at funcs_mem
+          rw [Nat.add_comm, Nat.add_right_cancel_iff] at depth_le
+
+          have aux := (aux ts).mpr (by
             constructor
-            . constructor
-              . exact ih.left
-              . exact ih_inner.left
-            constructor
-            . intro c c_mem
-              cases c_mem with
-              | inl c_mem => apply ih.right.left; exact c_mem
-              | inr c_mem => apply ih_inner.right.left; exact c_mem
-            . intro f f_mem
-              cases f_mem with
-              | inl f_mem => apply ih.right.right; exact f_mem
-              | inr f_mem => apply ih_inner.right.right; exact f_mem
-          . intro h
-            intro t t_mem
-            cases t_mem with
-            | inl t_mem =>
-              rw [t_mem, ih]
-              constructor
-              . exact h.left.left
-              constructor
-              . intro c c_mem
-                apply h.right.left
-                apply Or.inl
-                exact c_mem
-              . intro f f_mem
-                apply h.right.right
-                apply Or.inl
-                exact f_mem
-            | inr t_mem =>
-              apply ih_inner.mpr
-              . constructor
-                . exact h.left.right
-                constructor
-                . intro c c_mem
-                  apply h.right.left
-                  apply Or.inr
-                  exact c_mem
-                . intro f f_mem
-                  apply h.right.right
-                  apply Or.inr
-                  exact f_mem
-              . exact t_mem
-
-      constructor
-      . intro h
-        rw [List.mem_append] at h
-        cases h with
-        | inr h =>
-          rw [ih] at h
-          constructor
-          . apply Nat.le_succ_of_le
-            exact h.left
-          constructor
-          . exact h.right.left
-          . exact h.right.right
-        | inl h =>
-          simp only [List.mem_flatMap, List.mem_map] at h
-          rcases h with ⟨func, func_mem, ts, ts_mem, t_eq⟩
-          rw [← t_eq]
-          unfold List.attach at ts_mem
-          unfold List.attachWith at ts_mem
-          rw [List.mem_pmap] at ts_mem
-          rcases ts_mem with ⟨ts_val, ts_mem, ts_eq⟩
-          rw [mem_all_lists_of_length] at ts_mem
-
-          rw [GroundTerm.depth_func]
-          rw [GroundTerm.constants_func]
-          rw [GroundTerm.functions_func]
-
-          have this := (aux ts_val).mp (by
-            intro t t_mem
-            apply ts_mem.right
-            exact t_mem
+            . rw [List.all_eq_true]
+              intro t t_mem
+              rw [decide_eq_true_iff]
+              cases eq : (ts.map GroundTerm.depth).max? with
+              | none => rw [List.max?_eq_none_iff, List.map_eq_nil_iff] at eq; rw [eq] at t_mem; simp at t_mem
+              | some m =>
+                rw [eq, Option.getD_some, ← Nat.succ_eq_add_one] at depth_le
+                rw [List.max?_eq_some_iff] at eq
+                rw [← depth_le]
+                apply eq.right
+                rw [List.mem_map]
+                exists t
+            . grind
           )
 
-          rw [← ts_eq]
+          apply Or.inl
+          exists t_func
           constructor
-          . rw [Nat.add_comm]
-            apply Nat.succ_le_succ
-            cases eq : (ts_val.map GroundTerm.depth).max? with
-            | none => simp
-            | some m =>
-              rw [Option.getD_some, (ts_val.map GroundTerm.depth).max?_le_iff]
-              have depth_ts := List.all_eq_true.mp this.left
-              . simp only [decide_eq_true_iff] at depth_ts
-                intro d d_mem
-                rw [List.mem_map] at d_mem
-                rcases d_mem with ⟨t, t_mem, d_mem⟩
-                rw [← d_mem]
-                apply depth_ts
-                exact t_mem
-              . exact eq
-          constructor
-          . exact this.right.left
-          . intro func' func'_mem
-            rw [List.mem_cons] at func'_mem
-            cases func'_mem with
-            | inl func'_mem => rw [func'_mem]; exact func_mem
-            | inr func'_mem => apply this.right.right; exact func'_mem
-
-      . intro h
-        rw [List.mem_append]
-        simp only [List.mem_flatMap, List.mem_map]
-        rcases h with ⟨depth_le, consts_mem, funcs_mem⟩
-        rw [Nat.le_iff_lt_or_eq] at depth_le
-        cases depth_le with
-        | inl depth_le =>
-          apply Or.inr
-          rw [ih]
-          constructor
-          . apply Nat.le_of_lt_succ
-            exact depth_le
-          constructor
-          . exact consts_mem
-          . exact funcs_mem
-        | inr depth_le =>
-          cases eq : t with
-          | const _ => rw [eq] at depth_le; simp [GroundTerm.depth_const] at depth_le
-          | func t_func ts =>
-            rw [eq, GroundTerm.depth_func] at depth_le
-            rw [eq, GroundTerm.constants_func] at consts_mem
-            rw [eq, GroundTerm.functions_func] at funcs_mem
-            rw [Nat.add_comm, Nat.add_right_cancel_iff] at depth_le
-
-            have this := (aux ts).mpr (by
-              constructor
-              . rw [List.all_eq_true]
-                intro t t_mem
-                rw [decide_eq_true_iff]
-                cases eq : (ts.map GroundTerm.depth).max? with
-                | none => rw [List.max?_eq_none_iff, List.map_eq_nil_iff] at eq; rw [eq] at t_mem; simp at t_mem
-                | some m =>
-                  rw [eq, Option.getD_some, ← Nat.succ_eq_add_one] at depth_le
-                  rw [List.max?_eq_some_iff] at eq
-                  rw [← depth_le]
-                  apply eq.right
-                  rw [List.mem_map]
-                  exists t
-              constructor
-              . exact consts_mem
-              . intro func func_mem
-                apply funcs_mem
-                simp [func_mem]
-            )
-
-            apply Or.inl
-            exists t_func
-            constructor
-            . apply funcs_mem
-              simp
-
-            have ts_mem : ts ∈ all_lists_of_length (all_terms_limited_by_depth constants funcs depth.succ) t_func.arity := by
-              rw [mem_all_lists_of_length]
-              constructor
-              . have prop := t.property
-                unfold PreGroundTerm.arity_ok at prop
-                simp only [eq, GroundTerm.func, Bool.and_eq_true, beq_iff_eq] at prop
-                rw [List.length_unattach] at prop
-                exact prop.left
-              . intro t t_mem
-                apply this
-                exact t_mem
-
+          . apply funcs_mem; simp
+          . have ts_mem : ts ∈ all_lists_of_length (all_terms_limited_by_depth constants funcs depth.succ) t_func.arity := by grind
             exists ⟨ts, ts_mem⟩
             simp
 
